\documentclass{letter}
\usepackage{amsmath,amssymb}
\begin{document}

We are concerned with the variance of zero-centred normal distributed random variables transformed by the sine. Therefore we consider a mean of a particular transformed Wiener process $$f(t)=\mathbb{E}\left[\sin^2(cW_t)\right].$$

Knowing the derivatives  $$\frac{d}{dx}\sin^2(cx)=2c\sin(cx)\cos(cx)=c\sin(2cx)$$. $$\frac{d^2}{dx^2}\sin(x)^2 = 2c^2\cos(2cx),$$

we may apply Itô's lemma

\begin{equation*}
\begin{split}
\sin^2(cW_t) &= \int_0^t c\sin(2cW_s)dW_s + \frac{1}{2}\int_0^t 2c^2\cos(2cW_s)ds =\\
&=\int_0^t c\sin(2cW_s)dW_s + \int_0^t c^2\cos(2cW_s)ds.
\end{split}
\end{equation*}

Consequently

$$f(t)=c^2\int_0^t\mathbb{E}\left[\cos(2cW_s)\right]ds.$$

Now, consider

$$g(t,u)=\mathbb{E}\left[\cos(uW_t)\right].$$

Applying Itô's lemma we obtain

\begin{equation*}
\begin{split}
g(t,u)&=\mathbb{E}\left[\cos(u(W_s))\right]=\mathbb{E}\left[\frac{1}{2}\int_0^t-u^2\cos(uW_s)ds\right]=\\
&=-\frac{1}{2}u^2\int_0^t\mathbb{E}\left[\cos(uW_s)\right]ds=-\frac{1}{2}u^2 \int_0^tg(s,u)ds.
\end{split}
\end{equation*}

Thus

$$\frac{\partial g}{\partial t}\left(t,u\right)=-\frac{1}{2}u^2 g\left(t,u\right)$$
\newpage

and

$$g(t,u)=C(u)e^{-\frac{1}{2}u^2t}$$.

Since

$$g(0,u)=1$$

We have

$$C(u)=1$$

and thus that

$$g(t,u)=e^{-\frac{1}{2}u^2t}.$$

Thus

\begin{equation*}
\begin{split}
f(t) & =c^2\int_0^t\mathbb{E}\left[\cos(2cW_s)\right]ds=c^2\int_0^tg(t,2c)=\\
&=c^2\int_0^te^{-\frac{1}{2}4c^2t}=c^2\int_0^te^{-2c^2t}=\\
&=c^2\frac{e^{-2tc^2}-1}{-2c^2}=\frac{1-e^{-2c^2t}}{2}.
\end{split}
\end{equation*}

We can conclude that

$$\mathbb{E}\left[\sin(cZ)^2\right]=\frac{1-e^{-2c^2}}{2},$$

{\bf Calculation of \boldmath$\text{Var}\left[\cos(cZ)\right]$}

In the calculation of $\mathbb{E}[\sin(cZ)^2]$ we obtained two results that are relevant also for this calculation, that

$$\mathbb{E}[\cos(uW_t)]=e^{-\frac{1}{2}u^2t}$$

and the conclusion of the previous calculation, that

$$\mathbb{E}[\sin(cZ)^2]=\frac{1-e^{-2c^2}}{2}.$$

Because

$$\mathbb{E}\left[\sin(cZ)^2+\cos(cZ)^2\right]=1$$

it immediately follows that

\begin{equation*}
\begin{split}
\mathbb{E}\left[\cos(cZ)^2\right]&=1-\mathbb{E}\left[\sin(cZ)^2\right]=\\
&=1-\frac{1-e^{-2c^2}}{2}=\frac{1}{2}+\frac{1}{2}e^{-2c^2}.
\end{split}
\end{equation*}

Using that

$$\text{Var}\left[X\right]=\mathbb{E}\left[\left(X-\mathbb{E}\left[X\right]\right)^2\right]=\mathbb{E}[X^2]-\mathbb{E}[X]^2$$

we obtain

\begin{equation*}
\begin{split}
\text{Var}\left[\cos\left(cZ\right)\right]&=\frac{1}{2}+\frac{1}{2}e^{-2c^2}-\left(e^{-\frac{1}{2}c^2}\right)^2=\\
&=\frac{1}{2}+\frac{1}{2}e^{-2c^2}-e^{-c^2}
\end{split}
\end{equation*}

\end{document}